Microgrid/Microgrid_VC145.thy
@@ -1,6 +1,18 @@
 theory Microgrid_VC145
-imports MicrogridTheory
+imports MicrogridTheory Reflex
 begin
+
+definition inv3 :: "state\<Rightarrow>bool" where 
+"inv3 s = (\<forall> s1. substate s1 s 
+\<and> toEnvP s1 
+\<and> ((getVarBool s1 ''CycleCh''  
+  \<and> (getVarReal s1 ''Pl'' - getVarReal s1 ''Pwec'' < 1010*0.21))
+\<or> (getVarReal s1 ''SOC'' > 0.2 \<and> (getVarReal s1 ''Pl'' - getVarReal s1 ''Pwec'' > 550))) 
+\<and> getVarReal s1 ''Pdg'' > 0 
+\<longrightarrow> getVarReal s1 ''Pdg'' \<ge> 1010*0.6)"
+
+definition inv :: "state\<Rightarrow>bool" where
+"inv s \<equiv> inv3 s \<and> toEnvP s"
 
 lemma
  assumes base_inv:"(inv st0)"
@@ -10,28 +22,62 @@ lemma
  and st4:"(st4=(setVarReal st3 ''Pl'' Pl))"
  and st4_MainController_state:"(getPstate st4 ''MainController'')=''control''"
  and st4_if1:"((getVarReal st4 ''Pwec'') > (getVarReal st4 ''Pl''))=False"
- and st5:"(st5=(setPstate st4 ''RAEScharging'' ''''stop''''))"
+ and st5:"(st5=(setPstate st4 ''RAEScharging'' ''stop''))"
  and st6:"(st6=(setVarReal st5 ''RAESch'' (real 0)))"
- and st6_if1:"((getVarReal st6 ''SOC'') > 0.2)=False"
- and st7:"(st7=(setVarReal st6 ''RAESdisch'' (real 0)))"
- and st8:"(st8=(setPstate st7 ''RAESdischarging'' ''''stop''''))"
- and st8_if24:"(getPstate st8 ''GeneratorWork'' = ''stop'')=True"
- and st9:"(st9=(setPstate st8 ''GeneratorWork'' ''control''))"
- and st9_RAEScharging_state:"(getPstate st9 ''RAEScharging'')=''control''"
- and st9_if48:"(((getVarReal st9 ''SOC'') < (real 1)) \<and> (((getVarReal st9 ''Pwec'') - (getVarReal st9 ''Pl'')) > 250))=True"
- and st9_if50:"(((getVarReal st9 ''Pwec'') - (getVarReal st9 ''Pl'')) < 550)=False"
- and st10:"(st10=(setVarReal st9 ''RAESch'' 550))"
- and st11:"(st11=(setVarReal st10 ''Pwec_curt'' (((getVarReal st10 ''Pwec'') - (getVarReal st10 ''Pl'')) - 550)))"
- and st11_RAESdischarging_state:"(getPstate st11 ''RAESdischarging'')=''control''"
- and st11_if28:"(((getVarReal st11 ''Pl'') - (getVarReal st11 ''Pwec'')) > 250)=True"
- and st11_if29:"(((getVarReal st11 ''Pl'') - (getVarReal st11 ''Pwec'')) < 550)=True"
- and st12:"(st12=(setVarReal st11 ''RAESdisch'' ((getVarReal st11 ''Pl'') - (getVarReal st11 ''Pwec''))))"
- and st12_GeneratorWork_state:"(getPstate st12 ''GeneratorWork'')=''control''"
- and st12_if12:"(getVarBool st12 ''_dshcg_gen'')=True"
- and st13:"(st13=(setVarBool st12 ''_dshcg_gen'' False))"
- and st14:"(st14=(setVarReal st13 ''Pdg'' (((getVarReal st13 ''Pl'') - (getVarReal st13 ''Pwec'')) - 550)))"
- and st15:"(st15=(toEnv st14))"
- and st_final:"(st_final=st15)"
+ and st6_if0:"((getVarReal st6 ''SOC'') > 0.2)=True"
+ and st7:"(st7=(setPstate st6 ''RAESdischarging'' ''control''))"
+ and st7_RAEScharging_state:"(getPstate st7 ''RAEScharging'')=''stop''"
+ and st7_RAESdischarging_state:"(getPstate st7 ''RAESdischarging'')=''control''"
+ and st7_if16:"(((getVarReal st7 ''Pl'') - (getVarReal st7 ''Pwec'')) \<ge> 250)=True"
+ and st7_if18:"(((getVarReal st7 ''Pl'') - (getVarReal st7 ''Pwec'')) \<le> 550)=False"
+ and st8:"(st8=(setVarReal st7 ''RAESdisch'' 550))"
+ and st9:"(st9=(setVarBool st8 ''_dshcg_gen'' True))"
+ and st10:"(st10=(setPstate st9 ''GeneratorWork'' ''control''))"
+ and st10_GeneratorWork_state:"(getPstate st10 ''GeneratorWork'')=''control''"
+ and st10_if40:"(getVarBool st10 ''_dshcg_gen'')=True"
+ and st11:"(st11=(setVarBool st10 ''_dshcg_gen'' False))"
+ and st12:"(st12=(setVarReal st11 ''Pdg'' (((getVarReal st11 ''Pl'') - (getVarReal st11 ''Pwec'')) - 550)))"
+ and st13:"(st13=(toEnv st12))"
+ and st_final:"(st_final=st13)"
 shows "(inv st_final)"
+proof (simp only: inv_def;rule conjI)
+  show "inv3 st_final"
+  proof (simp only:inv3_def;rule allI;rule impI)
+  fix s1
+  assume assms1:"substate s1 st_final \<and>
+          toEnvP s1 \<and>
+          (getVarBool s1 ''CycleCh'' \<and>
+           getVarReal s1 ''Pl'' -
+           getVarReal s1 ''Pwec''
+           < 1010 * (21 / 10\<^sup>2) \<or>
+           2 / 10
+           < getVarReal s1 ''SOC'' \<and>
+           550
+           < getVarReal s1 ''Pl'' -
+             getVarReal s1 ''Pwec'') \<and>
+          0 < getVarReal s1 ''Pdg''"
+  then show "1010 * (6 / 10)\<le> getVarReal s1 ''Pdg''"
+  proof -
+  have "getVarReal st_final ''Pdg'' = (((getVarReal st_final ''Pl'') - (getVarReal st_final ''Pwec'')) - 550)" using assms by auto
+  moreover have "substate st_final st_final 
+              \<and> toEnvP st_final" using assms inv_def substate_refl by auto
+  moreover have "getVarReal st_final ''SOC'' > 0.2" using assms by auto
+  moreover have "getVarReal st_final ''Pl'' - getVarReal st_final ''Pwec'' > 550" using assms by auto
+  moreover have "getVarReal st_final ''Pdg'' > 0" using assms by auto
+  from calculation consider (a) "getVarReal st_final ''Pl'' - getVarReal st_final ''Pwec'' > 550 \<and> getVarReal st_final ''Pl'' - getVarReal st_final ''Pwec'' <1010*0.6 +550" 
+    | (b) "getVarReal st_final ''Pl'' - getVarReal st_final ''Pwec'' \<ge> 1010*0.6 +550" by linarith
+  then have "getVarReal st_final ''Pdg'' \<ge> 1010*0.6" 
+  proof cases
+    case a
+    then have "getVarReal st_final ''Pl'' - getVarReal st_final ''Pwec'' -550 < 1010*0.6" by auto
+    then have "getVarReal st_final ''Pdg'' < 1010*0.6" using calculation by auto
+    (*contradicts with provable statement*)
+    thus ?thesis by sorry
+  next
+    case b 
+    then have "getVarReal st_final ''Pl'' - getVarReal st_final ''Pwec'' -550 \<ge> 1010*0.6" by auto
+    thus ?thesis using calculation by auto
+  qed
+  
 
 end
