Microgrid/Microgrid_VC16.thy
@@ -17,10 +17,14 @@ lemma
  and st7_if0:"(((getVarReal st7 ''SOC'') < (real 1)) \<and> (((getVarReal st7 ''Pwec'') - (getVarReal st7 ''Pl'')) > 250))=True"
  and st7_if1:"(((getVarReal st7 ''Pwec'') - (getVarReal st7 ''Pl'')) < 550)=True"
  and st8:"(st8=(setVarReal st7 ''RAESch'' ((getVarReal st7 ''Pwec'') - (getVarReal st7 ''Pl''))))"
- and st8_RAESdischarging_state:"(getPstate st8 ''RAESdischarging'')=''stop''"
- and st8_GeneratorWork_state:"(getPstate st8 ''GeneratorWork'')=''stop''"
- and st9:"(st9=(toEnv st8))"
- and st_final:"(st_final=st9)"
+ and st8_RAESdischarging_state:"(getPstate st8 ''RAESdischarging'')=''control''"
+ and st8_if3:"(((getVarReal st8 ''Pl'') - (getVarReal st8 ''Pwec'')) > 250)=False"
+ and st9:"(st9=(setVarReal st8 ''RAESdisch'' (real 0)))"
+ and st9_if5:"(getPstate st9 ''GeneratorWork'' = ''stop'')=False"
+ and st10:"(st10=(setPstate st9 ''RAESdischarging'' ''''stop''''))"
+ and st10_GeneratorWork_state:"(getPstate st10 ''GeneratorWork'')=''stop''"
+ and st11:"(st11=(toEnv st10))"
+ and st_final:"(st_final=st11)"
 shows "(inv st_final)"
 
 end
